Util/Relation/Union.v
@@ -1,0 +1,94 @@
+(**
+CoLoR, a Coq library on rewriting and termination.
+See the COPYRIGHTS and LICENSE files.
+
+- Frederic Blanqui, 2007-02-05
+
+union of two wellfounded relations
+*)
+
+Set Implicit Arguments.
+
+Require Export Lexico.
+
+(***********************************************************************)
+(** R @ S << S @ R -> WF S -> WF (R# @ S) *)
+
+Section commut.
+
+Variables (A : Set) (R S : relation A) (commut : R @ S << S @ R).
+
+Lemma commut_SN_modulo : forall x, SN S x -> SN (R# @ S) x.
+
+Proof.
+induction 1. apply SN_intro. intros. deduce (commut_rtc commut H1).
+do 2 destruct H2. eapply SN_modulo. apply H0. apply H2. exact H3.
+Qed.
+
+Lemma commut_WF_modulo : WF S -> WF (R# @ S).
+
+Proof.
+unfold WF. intros. apply commut_SN_modulo. apply H.
+Qed.
+
+End commut.
+
+(***********************************************************************)
+(** R @ T << T -> WF T -> WF (T @ R#) *)
+
+Section absorb.
+
+Variables (A : Set) (R T : relation A) (absorb : R @ T << T).
+
+Lemma SN_modulo_r : forall x x', SN (T @ R#) x -> R# x x' -> SN (T @ R#) x'.
+
+Proof.
+intros. apply SN_intro. intros. apply (SN_inv H). do 2 destruct H1. exists x0.
+intuition. apply (comp_rtc_incl absorb). exists x'. intuition.
+Qed.
+
+Lemma absorb_SN_modulo_r : forall x, SN T x -> SN (T @ R#) x.
+
+Proof.
+induction 1. apply SN_intro. intros. apply SN_intro. intros.
+do 2 destruct H1. do 2 destruct H2.
+assert (T x0 x1). apply (comp_rtc_incl absorb). exists y. intuition.
+deduce (H0 _ H1). apply (SN_inv H6). exists x1. intuition.
+Qed.
+
+Lemma absorb_WF_modulo_r : WF T -> WF (T @ R#).
+
+Proof.
+unfold WF. intros. eapply absorb_SN_modulo_r. apply H.
+Qed.
+
+End absorb.
+
+(***********************************************************************)
+(** R @ S << S @ R -> WF R -> WF S -> WF (R U S) *)
+
+Section union1.
+
+Variables (A : Set) (R S : relation A) (commut : R @ S << S @ R).
+
+Lemma WF_union : WF R -> WF S -> WF (R U S).
+
+Proof.
+intros. eapply WF_incl. apply tc_incl. eapply WF_incl. apply tc_union.
+set (T := R# @ S). set (gt1 := T! @ R#). set (gt2 := R!).
+eapply WF_incl. apply union_commut.
+eapply WF_incl. apply lex'_intro. apply lex'_WF.
+(* WF gt1 *)
+unfold gt1. apply absorb_WF_modulo_r. trans (R# @ T!). comp.
+apply rtc_incl. unfold T. apply rtc_comp_modulo.
+apply WF_tc. unfold T. apply commut_WF_modulo. exact commut. exact H0.
+(* WF gt2 *)
+unfold gt2. apply WF_tc. exact H.
+(* transitive gt2 *)
+apply trans_intro. unfold gt2. apply tc_idem.
+(* gt2 @ gt1 << gt1 *)
+unfold gt1, gt2. trans ((R! @ T!) @ R#). apply comp_assoc'. comp.
+trans (R# @ T!). comp. apply tc_incl_rtc. unfold T. apply rtc_comp_modulo.
+Qed.
+
+End union1.
